\documentclass[paper=a4, fontsize=11pt]{scrartcl} % A4 paper and 11pt font size

\usepackage{amssymb}
\usepackage{siunitx}
\usepackage{amsmath,amsfonts,amsthm} % Math packages3
\usepackage{scalerel}

\begin{document}

$$x_{t+1} = x_t + v * cos(\psi_t) * dt$$

$$y_{t+1} = y_t + v * sin(\psi_t) * dt$$

$$\psi_{t+1} = \psi_{t} + \frac{v_t}{L_f} * \delta_t * dt $$

$$ v_{t+1} = v_t + a_t * dt $$

$$ cte_{t+1} = y_t - f(x_t) + (v_t * sin(e_{\psi_{\scaleto{t}{3pt}}}) * dt)$$

$$ e_{\psi_{\scaleto{t+1}{3pt}}} = \psi_t - \arctan{(f'(x_t))} + (\frac{v_t}{L_f} * \delta_t * dt)$$

$$ cost_t = \sqrt{(X_{dst} - X_t)^2 + (Y_{dst} - Y_t)^2}$$

$$ cost_t = (v_t - v_{reference})^2$$

$$ cost_t = \delta_t^2$$

$$ cost_t = (\delta_{t+1} - \delta_t)^2 + (a_{t+1} - a_t)^2 $$

$$ J = \sum_{t=1}^N cte_t^2 + e_{\psi_{\scaleto{t}{3pt}}}^2 + \delta^2 + [(\delta_t - \delta_{t-1}) ^2 + (a_t - a_{t-1})^2] + (v_t - v_{reference})^2) $$

\begin{equation*}
\begin{aligned}
& \underset{a, \delta}{\text{minimize}}
& & cost_{x_{\scaleto{1}{3pt}}, y_{\scaleto{1}{3pt}}, v_{\scaleto{1}{3pt}}, \psi_{\scaleto{1}{3pt}}, cte_{\scaleto{1}{3pt}}, e_{\psi_{\scaleto{1}{3pt}}}, f}(a, \delta)\\
& \text{subject to}
& & \delta \in \mathbb{R}^{N-1} \\
& & & a \in \mathbb{R}^{N-1} \\
& & & \ang{-25} \preceq \delta \preceq \ang{25} \\
& & & -1 \preceq a \preceq 1 \\
\end{aligned}
\end{equation*}

\end{document}